examples/combinatorics.dfy
@@ -1,0 +1,291 @@
+
+module Combinatorics {
+
+    function Factorial(n: int): int
+        requires n >= 0
+        ensures Factorial(n) == if n == 0 then 1 else n * Factorial(n - 1)
+    {
+        if n <= 0 then 1 else n * Factorial(n - 1)
+    }
+
+    function Numbers(): set<int> {
+        {0,1,2,3,4,5,6,7,8,9}
+    }
+
+    function ToPairB<A(==),B(==)>(xs: set<A>, y: B): set<(A,B)> {
+        set a | a in xs :: (a, y)
+    }
+
+    function ToPairA<A(==),B(==)>(x: A, ys: set<B>): set<(A,B)> {
+        set b | b in ys :: (x, b)
+    }
+
+    function SevenTuples<A>(xs: set<A>): set<(A,A,A,A,A,A,A)> {
+        set a1, a2, a3, a4, a5, a6, a7 | a1 in xs && a2 in xs && a3 in xs && a4 in xs && a5 in xs && a6 in xs && a7 in xs :: (a1, a2, a3, a4, a5, a6, a7)
+    }
+
+    function ThreeTuples<A>(xs: set<A>): set<(A,A,A)> {
+        set a1, a2, a3 | a1 in xs && a2 in xs && a3 in xs :: (a1, a2, a3)
+    }
+
+    lemma ThreeTuplesSize<A>(xs: set<A>)
+        ensures |ThreeTuples(xs)| == |xs| * |xs| * |xs|
+    {
+        CrossSize(xs, xs);
+        CrossSize(xs, Cross(xs,xs));
+        BijectionImpliesEqualCardinality(
+                ThreeTuples(xs),
+                Cross(xs, Cross(xs, xs)),
+                (triple: (A, A, A)) => (triple.0, (triple.1, triple.2)),
+                (pair: (A, (A, A))) => (pair.0, pair.1.0, pair.1.1)
+            );
+        // assert |ThreeTuples(xs)| == |xs| * |xs| * |xs|;
+    }
+
+    function Tuples<A>(xs: set<A>): set<(A,A)> {
+        set a1, a2 | a1 in xs && a2 in xs :: (a1, a2)
+    }
+
+    lemma ToPairASize<A,B>(x: A, ys: set<B>)
+        ensures |ToPairA(x, ys)| == |ys|
+    {
+        if |ys| == 0 {
+            assert |ToPairA(x, ys)| == 0;
+        } else {
+            var b :| b in ys;
+            assert forall b1 :: b1 in ys ==> ((x, b1) in ToPairA(x, ys));
+            ToPairASize(x, ys - {b});
+            assert ToPairA(x, ys) == {(x, b)} + ToPairA(x, ys - {b});
+            assert |ToPairA(x, ys)| == |ys|;
+        }
+    }
+
+    lemma ToPairSize<A,B>(xs: set<A>, y: B)
+        ensures |ToPairB(xs, y)| == |xs|
+    {
+        if |xs| == 0 {
+            assert |ToPairB(xs, y)| == 0;
+        } else {
+            var a :| a in xs;
+            assert forall a1 :: a1 in xs ==> ((a1, y) in ToPairB(xs, y));
+            ToPairSize(xs - {a}, y);
+            assert ToPairB(xs, y) == {(a, y)} + ToPairB(xs - {a}, y);
+            assert |ToPairB(xs, y)| == |xs|;
+        }
+    }
+
+    function Cross<A,B>(a: set<A>, b: set<B>): set<(A,B)> {
+        set a1, b1 | a1 in a && b1 in b :: (a1, b1)
+    }
+
+    lemma CrossTuplesEqual<A>(a: set<A>) 
+        ensures Cross(a, a) == Tuples(a)
+    {
+        // if |a| == 0 {
+        //     assert Cross(a, a) == {};
+        // } else {
+        //     var a1 :| a1 in a;
+        //     CrossTuplesEqual(a - {a1});
+        //     assert Cross(a, a) == Cross(a - {a1}, a) + ToPairB(a - {a1}, a1);
+        //     assert Cross(a, a) == Tuples(a - {a1}) + ToPairB(a - {a1}, a1);
+        // }
+    }
+
+
+    lemma CrossPlusOne<A,B>(a: set<A>, b: set<B>, x: B)
+        requires x !in b
+        ensures Cross(a, b + {x}) == Cross(a, b) + ToPairB(a, x)
+        decreases |b|
+    {
+    }
+
+    lemma CrossPlusOneA<A,B>(a: set<A>, b: set<B>, x: A)
+        requires x !in a
+        ensures Cross(a + {x}, b) == Cross(a, b) + ToPairA(x, b)
+        decreases |a|
+    {
+    }
+
+    lemma CrossSizePlusOneA<A,B>(a: set<A>, b: set<B>, x: A)
+        // requires |b| > 0 
+        requires x !in a
+        ensures |Cross(a + {x}, b)| == |Cross(a, b)| + |b|
+        decreases |a|
+    {
+        if |a| == 0 && |b| == 0 {
+            assert |Cross(a + {x}, b)| == 0;
+        } else if |a| == 0 {
+            assert Cross(a + {x}, b) == ToPairA(x, b);
+            ToPairASize(x, b);
+        }else if |b| == 0 {
+            assert |Cross(a, b)| == 0;
+        } else {
+            CrossPlusOneA(a, b, x);
+            ToPairASize(x, b);
+            assert |Cross(a + {x}, b)| == |Cross(a, b)| + |b|;
+        }
+    }
+    
+    
+    lemma CrossSizePlusOne<A,B>(a: set<A>, b: set<B>, x: B)
+        // requires |a| > 0 
+        requires x !in b
+        ensures |Cross(a, b + {x})| == |Cross(a, b)| + |a|
+        decreases |b|
+    {
+        if |a| == 0 && |b| == 0 {
+            assert |Cross(a, b + {x})| == 0;
+        } else  if |a| == 0 {
+            assert |Cross(a, b)| == 0;
+        }else if |b| == 0 {
+            assert Cross(a, b + {x}) == ToPairB(a, x);
+            ToPairSize(a, x);
+            assert |Cross(a, b + {x})| == |a|;
+        } else {
+            CrossPlusOne(a, b, x);
+            ToPairSize(a, x);
+            assert |Cross(a, b + {x})| == |Cross(a, b)| + |a|;
+        }
+    }
+
+    lemma CrossSize<A, B>(a: set<A>, b: set<B>)
+        ensures |Cross(a, b)| == |a| * |b|
+        decreases |a| + |b|
+    {
+        if |a| == 0  {
+            assert |Cross(a, b)| == 0;
+        }else if |a| == 1 {
+            var a1 :| a1 in a;
+            CrossSizePlusOneA({}, b, a1);
+            assert |a-{a1}| == 0;
+            assert a == {} + {a1};
+            assert Cross(a, b) == ToPairA(a1, b);
+        } else {
+            var a1 :| a1 in a;
+            // var b1 :| b1 in b;
+            CrossPlusOneA(a - {a1}, b, a1);
+            // CrossPlusOne(a, b - {b1}, b1);
+            CrossSizePlusOneA(a - {a1}, b, a1);
+            // CrossSizePlusOne(a, b - {b1}, b1);
+            CrossSize(a - {a1}, b);
+            // CrossSize(a, b - {b1});
+            calc {
+                |Cross(a - {a1}, b)| + |b|;
+                |a - {a1}| * |b| + |b|;
+                (|a| - 1) * |b| + |b|;
+                |a| * |b| - |b| + |b|;
+                |a| * |b|;
+            }
+            // calc {
+            //     |Cross(a, b - {b1})| + |a|;
+            //     |a| * (|b| - 1) + |a|;
+            //     |a| * |b| - |a| + |a|;
+            //     |a| * |b|;
+            // }
+            assert Cross(a, b) == Cross(a - {a1}, b) + ToPairA(a1, b);
+            ToPairASize(a1, b);
+            assert |Cross(a, b)| == |Cross(a - {a1}, b)| + |b|;
+        }
+    }
+    datatype IteratedSet<A(==)> = Base(a: A) | Pair(left: A, right: IteratedSet<A>)
+
+    // function CrossIteratedSet<A>(As: set<A>, s: IteratedSet<A>): IteratedSet<A> {
+
+    // }
+
+    lemma TripleSelectionEqualsCrossCross<T(==)>(s: set<T>)
+        ensures (set a1, a2, a3 | a1 in s && a2 in s && a3 in s :: (a1, (a2, a3))) == Cross(s, Cross(s, s))
+    {
+    }
+
+    lemma TripleSelectionEqualsCrossCross2<T(==)>(s: set<T>)
+        ensures |(set a1, a2, a3 | a1 in s && a2 in s && a3 in s :: (a1, (a2, a3)))| == |Cross(s, Cross(s, s))|
+    {
+        TripleSelectionEqualsCrossCross(s);
+    }
+
+    lemma BijectionImpliesEqualCardinality<T(==), U(==)>(xs: set<T>, ys: set<U>, f: T -> U, g: U -> T)
+        requires forall x :: x in xs ==> g(f(x)) == x
+        requires forall y :: y in ys ==> f(g(y)) == y
+        requires forall x :: x in xs ==> f(x) in ys
+        requires forall y :: y in ys ==> g(y) in xs
+        ensures |xs| == |ys|
+    {
+        if xs == {} {
+            assert ys == {};
+            assert |xs| == 0;
+            assert |ys| == 0;
+        }else if |xs| == 1 {
+            var x :| x in xs;
+            assert |xs-{x}| == 0;
+            // assert f(x) in ys;
+            // assert g(f(x)) == x;
+            assert ys == {f(x)};
+            //  by {
+            //     // if y :| y in ys && f(x) != y {
+            //     //     // assert g(y) in xs;
+            //     //     assert false;
+            //     // }
+            // }
+            assert |ys| == 1;
+        } else {
+            var x :| x in xs;
+            BijectionImpliesEqualCardinality(xs - {x}, ys - {f(x)}, f, g);
+            
+            assert |xs| == |ys|;
+        }
+    }
+
+    lemma TripleSelectionEqualsCrossCross3<T(==)>(s: set<T>)
+        ensures |(ThreeTuples(s))| == |Cross(s, Cross(s, s))|
+    {
+        var target := set a1, a2, a3 | a1 in s && a2 in s && a3 in s :: (a1, a2, a3);
+        // TripleSelectionEqualsCrossCross(s);
+        // TripleSelectionEqualsCrossCross2(s);
+        // forall p | p in Cross(s, Cross(s, s)) 
+        //     ensures (p.0, p.1.0, p.1.1) in target
+        // {
+        //     assert (p.0, p.1.0, p.1.1) in target;
+        // }
+
+        // forall p | p in target 
+        //     ensures (p.0, (p.1, p.2)) in Cross(s, Cross(s, s))
+        // {
+        //     assert (p.0, (p.1, p.2)) in Cross(s, Cross(s, s));
+        // }
+        BijectionImpliesEqualCardinality(
+            Cross(s, Cross(s, s)),
+            target,
+            (pair: (T, (T, T))) => (pair.0, pair.1.0, pair.1.1),
+            (triple: (T, T, T)) => (triple.0, (triple.1, triple.2))
+        );
+        assert |target| == |Cross(s, Cross(s, s))|;
+    }
+
+
+    lemma Test() {
+        var twos := Cross(Numbers(), Numbers());
+        CrossSize(Numbers(), Numbers());
+        assert |twos| == 10 * 10;
+        var threes := Cross(Numbers(), twos);
+        var threes2 := set triple | triple in threes :: (triple.0, triple.1.0, triple.1.1);
+        var threes3 := set a1, a2, a3 | a1 in Numbers() && a2 in Numbers() && a3 in Numbers() :: (a1, a2, a3);
+        CrossSize(Numbers(), twos);
+        assert |threes| == 10 * 10 * 10;
+        // assert |threes2| == 10 * 10 * 10;
+        // assert |threes2| == 10 * 10 * 10;
+        // assert |threes3| == 10 * 10 * 10;
+        // assert threes2 == threes3;
+    }
+
+    // function telephoneNumbers(): set<seq<int>> {
+    //     set x | |x| == 7 && forall i :: 0 <= i < |x| ==> (x[i] in Numbers()) 
+    // }
+
+    // function BinomialCoefficient(n: int, k: int): int
+    //     requires n >= 0 && k >= 0 && k <= n
+    //     ensures BinomialCoefficient(n, k) == Factorial(n) / (Factorial(k) * Factorial(n - k))
+    // {
+    //     if k == 0 || k == n then 1 else BinomialCoefficient(n - 1, k - 1) + BinomialCoefficient(n - 1, k)
+    // }
+}
